qr

QR/Basics.ec
@@ -4,42 +4,43 @@ require import AllCore DBool Bool List Distr Aux.
 require  GenericSigmaProtocol.
 
 
-require import ZModP.
-clone include ZModRing.         (* must use ring since in ZModField QR is efficiently computable *)
-(* import DZmodP. *)
+require import ZModP.           (* standard library formalization of zmod fields, rings, etc.  *)
 
-abbrev invertible = unit.           (* more intuitive synonym *)
+clone include ZModRing.         (* for FiatShamir we must use ring since in ZModField QR is efficiently computable *)
 
-type qr_prob = zmod.
+abbrev invertible = unit.       (* more intuitive synonym *)
+
+
+(* uniform distribution of invertible elements, could be constructed from DZmodP   *)
+op zmod_distr : zmod distr.
+axiom d_prop0 : is_uniform zmod_distr.
+axiom d_prop3 (r : zmod) :  invertible r => r \in zmod_distr.
+axiom d_prop4 r : r \in zmod_distr => invertible r.
+axiom d_prop5 : weight zmod_distr = 1%r.
+
+
+(* synonyms for readability *)
+type qr_stat = zmod.
 type qr_wit  = zmod.
 type qr_com  = zmod.
 type qr_resp = zmod.
 
 
-op ZNS_dist :  (zmod * zmod) distr.
-
-axiom d_prop0  : is_uniform ZNS_dist.
-axiom d_prop1 r rr :  (r, rr) \in ZNS_dist => r * r = rr.
-axiom d_prop3 (r rr : zmod) :  r * r = rr => (r, rr) \in ZNS_dist.
-axiom d_prop4  r rr :  (r, rr) \in ZNS_dist => unit rr.
-axiom d_prop5 : weight (ZNS_dist) = 1%r.
+op completeness_relation (s:qr_stat) (w:qr_wit) = s = (w * w) /\ invertible s.
+op soundness_relation = completeness_relation.
+op zk_relation = completeness_relation.
 
 
+op verify_transcript (p: qr_stat) (x : qr_com * bool * qr_resp) : bool =
+ let c = x.`1 in 
+ let b = x.`2 in
+ let r = x.`3 in   
+ unit c /\ unit p /\ if b then c * p = r * r 
+                          else c = r * r.
 
-op completeness_relation = fun Ny w => Ny = (w * w) /\ invertible Ny.
-op soundness_relation    = fun Ny w => Ny = (w * w) /\ invertible Ny.
-op zk_relation           = fun Ny w => Ny = (w * w) /\ invertible Ny.
-
-
-(* Honest Vrifier  *)
-op qr_verify (p : qr_prob) (c : qr_com) (b : bool) (r : qr_resp) : bool =
-  if b then unit c /\ unit p /\ c * p = r * r 
-  else unit c /\ c = r * r.
-
-op verify_transcript = fun p (x : qr_com * bool * qr_resp) => qr_verify p x.`1 x.`2 x.`3.
 
 clone export GenericSigmaProtocol as FiatShamir with 
-  type statement       <- qr_prob,
+  type statement       <- qr_stat,
   type commitment      <- qr_com,  
   type witness         <- qr_wit,
   type response        <- qr_resp,
@@ -51,44 +52,20 @@ clone export GenericSigmaProtocol as FiatShamir with
   op zk_relation           <- zk_relation.
 
 
-
-lemma qr_prop1 (x : zmod) : unit x => x * (inv x)  = one. smt. qed.
-lemma qr_prop2 (x y w : zmod) : unit y => y = w * w => unit w. smt. qed.
-lemma qr_prop3 (w : zmod) : unit  w => inv (w * w) = (inv w) * (inv w). smt. qed.
-lemma qr_prop11 (x : zmod) : unit x => (inv x) * x = one. smt. qed.
-lemma qr_prop5 (x y r : zmod) : in_language completeness_relation x 
-  => !in_language completeness_relation y => unit y => x * y  <> r * r.
-progress.
-elim H. progress. 
-case (x * y = r * r). elim H.
-move => H xinv.
-pose w := witness.
-rewrite  H. 
-have iw : invertible witness.  smt.
-move => eq.
-have eq2 :  (inv w) * w * w * y = (inv w) * r * r. smt.
-have eq3 :  w * y = (inv w) * r * r. smt.
-clear eq2 eq.
-have eq4 :  (inv w) * w * y = ((inv w) * r) * (inv w) * r. smt.
-have eq5 :  y = ((inv w) * r) * ((inv w) * r). smt.
-apply H0. exists (inv w * r). split.
-apply eq5. auto.
-auto.
-qed.
-
-
-
-(* Honest Prover  *)
+(* Honest Prover *)
 module HP : HonestProver = {
-  var r,rr, y, w : zmod
+  var r, y, w : zmod
 
-  proc commitment(Ny1 : qr_prob, w1 : qr_wit) : zmod = {  
+  proc commitment(Ny1 : qr_stat, w1 : qr_wit) : zmod = {  
     (y,w) <- (Ny1, w1);
-    (r,rr) <$ ZNS_dist;
-    return rr;
+    r <$ zmod_distr;
+    return r * r;
   }
 
   proc response(b : bool) : qr_resp = {
     return r * (if b then w else one);
  } 
 }.
+
+(* Honest Verifier is derived automatically from "challenge_set" and "verify_transcript" *)
+print HV.
