QR/SpecialSoundness.ec
@@ -3,15 +3,13 @@ require import AllCore DBool Bool List Distr.
 require import Aux Permutation Basics.
 
 
-(* t1 for true run, t2 for false run *)
-op my_extract (p : qr_prob) (t1 t2 : transcript) : qr_wit
- = ((inv  t2.`3) * t1.`3) .
-
-op special_soundness_extract (p : qr_prob) (t1 t2 : transcript): qr_wit
- = if t1.`2 then my_extract p t1 t2 else my_extract p t2 t1.
+op special_soundness_extract (p : qr_stat) (t1 t2 : transcript): qr_wit
+ = let (c1,ch1,r1) = t1 in
+   let (c2,ch2,r2) = t2 in
+   if ch1 then  (inv r2) * r1 else (inv r1) * r2.
 
 
-lemma perfect_special_soundness (statement:qr_prob) 
+lemma perfect_special_soundness (statement:qr_stat) 
  (transcript1 transcript2: transcript):
         valid_transcript_pair statement transcript1 transcript2 =>
    soundness_relation statement 
@@ -23,12 +21,25 @@ case (transcript2.`2).
 smt.
 rewrite /qr_verify. simplify.
 progress. 
-rewrite /special_soundness_extract. 
-rewrite H0. simplify. rewrite /my_extract.
-rewrite /IsSqRoot.
+rewrite /special_soundness_extract.  
 have -> : statement
    = ((inv  transcript1.`1))  * (transcript1.`3) * (transcript1.`3 ). smt.
 rewrite H1.
-rewrite H6. smt. 
+rewrite H7. smt. 
+rewrite /valid_transcript_pair. rewrite /verify_transcript.
+case (!transcript2.`2). 
+smt.
+move => z.
+have ->: transcript2.`2 = true.  smt.
+clear z.
+move => z.
+have zz: transcript1.`2 = false. smt.
+clear z.
+rewrite /qr_verify. simplify.
+progress. 
+rewrite /special_soundness_extract. 
+simplify. rewrite /my_extract.
+have -> : statement
+   = ((inv  transcript2.`1))  * (transcript2.`3) * (transcript2.`3 ). smt.
 smt.   
 qed.
